disable several proofs to move to nightly

Arm/SeparateProofs.lean
@@ -4,18 +4,18 @@ Released under Apache 2.0 license as described in the file LICENSE.
 Author(s): Shilpi Goel
 -/
 import Arm.Memory
-import Auto
+-- import Auto
 
 -- In this file, we have memory-related proofs that depend on auto.
 
-set_option auto.smt true
-set_option auto.smt.trust true
-set_option auto.smt.timeout 20 -- seconds
-set_option auto.smt.save true
--- set_option trace.auto.smt.printCommands true
-set_option trace.auto.smt.result true -- Print the SMT solver's output
-set_option trace.auto.smt.model true  -- Print the counterexample, if any
-set_option trace.auto.smt.proof false -- Do not print the proof.
+-- set_option auto.smt true
+-- set_option auto.smt.trust true
+-- set_option auto.smt.timeout 20 -- seconds
+-- set_option auto.smt.save true
+-- -- set_option trace.auto.smt.printCommands true
+-- set_option trace.auto.smt.result true -- Print the SMT solver's output
+-- set_option trace.auto.smt.model true  -- Print the counterexample, if any
+-- set_option trace.auto.smt.proof false -- Do not print the proof.
 
 ----------------------------------------------------------------------
 
@@ -31,41 +31,41 @@ theorem n_minus_1_lt_2_64_1 (n : Nat)
   (n - 1)#64 < (2 ^ 64 - 1)#64 := by
   refine BitVec.val_bitvec_lt.mp ?a
   simp [BitVec.bitvec_to_nat_of_nat]
-  have : n - 1 < 2 ^ 64 := by exact tsub_lt_of_lt h2
+  have : n - 1 < 2 ^ 64 := by omega
   simp_all [Nat.mod_eq_of_lt]
   exact Nat.sub_lt_left_of_lt_add h1 h2
 
 -- (FIXME) Prove for all bitvector widths, without using auto.
-set_option auto.smt.savepath "/tmp/BitVec.add_sub_self_left_64.smt2" in
+-- set_option auto.smt.savepath "/tmp/BitVec.add_sub_self_left_64.smt2" in
 theorem BitVec.add_sub_self_left_64 (a m : BitVec 64) :
   a + m - a = m := by
-  auto
+  sorry -- auto
 
 -- (FIXME) Prove for all bitvector widths, without using auto.
-set_option auto.smt.savepath "/tmp/BitVec.add_sub_self_right_64.smt2" in
+-- set_option auto.smt.savepath "/tmp/BitVec.add_sub_self_right_64.smt2" in
 theorem BitVec.add_sub_self_right_64 (a m : BitVec 64) :
   a + m - m = a := by
-  auto
+  sorry -- auto
 
 -- (FIXME) Prove for all bitvector widths, without using auto.
-set_option auto.smt.savepath "/tmp/BitVec.add_sub_add_left.smt2" in
+-- set_option auto.smt.savepath "/tmp/BitVec.add_sub_add_left.smt2" in
 theorem BitVec.add_sub_add_left (a m n : BitVec 64) :
   a + m - (a + n) = m - n := by
-  auto
+  sorry -- auto
 
 -- (FIXME) Prove without auto using general assoc/comm BitVec lemmas.
-set_option auto.smt.savepath "/tmp/BitVec.sub_of_add_is_sub_sub.smt2" in
+-- set_option auto.smt.savepath "/tmp/BitVec.sub_of_add_is_sub_sub.smt2" in
 theorem BitVec.sub_of_add_is_sub_sub (a b c : BitVec 64) :
   (a - (b + c)) = a - b - c := by
-  auto
+  sorry -- auto
 
 -- (FIXME) Prove without auto using general assoc/comm BitVec lemmas.
-set_option auto.smt.savepath "/tmp/BitVec.add_of_sub_sub_of_add.smt2" in
+-- set_option auto.smt.savepath "/tmp/BitVec.add_of_sub_sub_of_add.smt2" in
 theorem BitVec.add_of_sub_sub_of_add (a b c : BitVec 64) :
   (a + b - c) = a - c + b := by
-  auto
+  sorry -- auto
 
-set_option auto.smt.savepath "/tmp/nat_bitvec_sub1.smt2" in
+-- set_option auto.smt.savepath "/tmp/nat_bitvec_sub1.smt2" in
 theorem nat_bitvec_sub1 (x y : BitVec 64)
   (_h : y.toNat <= x.toNat) :
   (x - y).toNat = (x.toNat - y.toNat) % 2^64 := by
@@ -77,7 +77,7 @@ theorem nat_bitvec_sub1 (x y : BitVec 64)
   -- Let's reduce 2^64 to a constant for SMT solvers.
   simp (config := {ground := true}) only
   rw [Nat.mod_eq_sub_mod]
-  auto; auto
+  sorry; sorry -- auto; auto
 
 theorem nat_bitvec_sub2 (x y : Nat)
   (h : y <= x) (xub : x < 2^64) :
@@ -91,18 +91,23 @@ theorem nat_bitvec_sub2 (x y : Nat)
   have xmyub : x - y < 2^64 := calc
     x - y ≤ x := Nat.sub_le x y
     _ < _ := xub
+  simp at xmyub
   rw [Nat.mod_eq_of_lt xmyub]
+  simp at xub yub
   conv =>
-    pattern (x % 2 ^ 64 - y % 2 ^ 64)
+    pattern (x % 18446744073709551616 - y % 18446744073709551616)
     rw [Nat.mod_eq_of_lt xub, Nat.mod_eq_of_lt yub]
   rw [Nat.mod_eq_of_lt xmyub]
   simp [BitVec.bitvec_to_nat_of_nat]
+  simp at xub yub
   rw [Nat.mod_eq_of_lt xub, Nat.mod_eq_of_lt yub]
   exact h
 
 theorem addr_add_one_add_m_sub_one  (n : Nat) (addr : BitVec 64)
   (h_lb : Nat.succ 0 ≤ n) (h_ub : n + 1 ≤ 2 ^ 64) :
   (addr + 1#64 + (n - 1)#64) = addr + n#64 := by
+  sorry
+/-
   have h_ub' : n < 2^64 := by exact h_ub
   rw [nat_bitvec_sub2 n 1 h_lb h_ub']
   ext
@@ -113,17 +118,18 @@ theorem addr_add_one_add_m_sub_one  (n : Nat) (addr : BitVec 64)
   rw [←Nat.add_sub_assoc h_lb]
   simp only [Nat.succ_add_sub_one]
   done
+-/
 
 ----------------------------------------------------------------------
 ---- mem_subset ----
 
 -- (FIXME) As for Dec. 2023, lean-auto cannot resolve <[=] to
 -- Std.BitVec.ul[t/e].
-def lt_and_bitvec_lt (x y : BitVec n) : x < y ↔ Std.BitVec.ult x y := by
-  simp [LT.lt, Std.BitVec.ult]
+theorem lt_and_bitvec_lt (x y : BitVec n) : x < y ↔ Std.BitVec.ult x y := by
+  sorry -- simp [LT.lt, Std.BitVec.ult]
 
-def le_and_bitvec_le (x y : BitVec n) : x <= y ↔ Std.BitVec.ule x y := by
-  simp [LE.le, Std.BitVec.ule]
+theorem le_and_bitvec_le (x y : BitVec n) : x <= y ↔ Std.BitVec.ule x y := by
+  sorry -- simp [LE.le, Std.BitVec.ule]
 
 def mem_overlap_for_auto (a1 a2 b1 b2 : BitVec 64) : Bool :=
   Std.BitVec.ule (b1 - a1) (a2 - a1) ||
@@ -135,6 +141,7 @@ theorem mem_overlap_and_mem_overlap_for_auto :
   mem_overlap a1 a2 b1 b2 = mem_overlap_for_auto a1 a2 b1 b2 := by
   unfold mem_overlap mem_overlap_for_auto
   simp [le_and_bitvec_le]
+  sorry
 
 def mem_subset_for_auto (a1 a2 b1 b2 : BitVec 64) : Bool :=
   ((b2 - b1) = 18446744073709551615#64) ||
@@ -144,56 +151,56 @@ def mem_subset_for_auto (a1 a2 b1 b2 : BitVec 64) : Bool :=
 theorem mem_subset_and_mem_subset_for_auto :
   mem_subset a1 a2 b1 b2 = mem_subset_for_auto a1 a2 b1 b2 := by
   unfold mem_subset mem_subset_for_auto
-  have : 2^64 - 1 = 18446744073709551615 := by decide
-  simp [le_and_bitvec_le, this]
+  simp [le_and_bitvec_le]
+  sorry
 
-set_option auto.smt.savepath "/tmp/mem_subset_refl.smt2" in
+-- set_option auto.smt.savepath "/tmp/mem_subset_refl.smt2" in
 theorem mem_subset_refl : mem_subset a1 a2 a1 a2 := by
   simp [mem_subset_and_mem_subset_for_auto]
-  auto d[mem_subset_for_auto]
+  sorry -- auto d[mem_subset_for_auto]
 
-set_option auto.smt.savepath "/tmp/mem_subsets_overlap.smt2" in
+-- set_option auto.smt.savepath "/tmp/mem_subsets_overlap.smt2" in
 theorem mem_subsets_overlap (h : mem_subset a1 a2 b1 b2) :
   mem_overlap a1 a2 b1 b2 := by
   revert h
   simp [mem_subset_and_mem_subset_for_auto, mem_overlap_and_mem_overlap_for_auto]
-  auto d[mem_overlap_for_auto, mem_subset_for_auto]
+  sorry -- auto d[mem_overlap_for_auto, mem_subset_for_auto]
 
-set_option auto.smt.savepath "/tmp/mem_subset_eq.smt2" in
+-- set_option auto.smt.savepath "/tmp/mem_subset_eq.smt2" in
 theorem mem_subset_eq : mem_subset a a b b = (a = b)  := by
   simp [mem_subset_and_mem_subset_for_auto]
-  auto d[mem_subset_for_auto]
+  sorry -- auto d[mem_subset_for_auto]
 
-set_option auto.smt.savepath "/tmp/mem_subset_first_address.smt2" in
+-- set_option auto.smt.savepath "/tmp/mem_subset_first_address.smt2" in
 theorem mem_subset_first_address (h : mem_subset a b c d) :
   mem_subset a a c d := by
   revert h
   simp_all [mem_subset_and_mem_subset_for_auto, le_and_bitvec_le, lt_and_bitvec_lt]
-  auto d[mem_subset_for_auto]
+  sorry -- auto d[mem_subset_for_auto]
 
-set_option auto.smt.savepath "/tmp/mem_subset_one_addr_neq.smt2" in
+-- set_option auto.smt.savepath "/tmp/mem_subset_one_addr_neq.smt2" in
 theorem mem_subset_one_addr_neq (h1 : a ≠ b1)
   (h : mem_subset a a b1 b2) :
   mem_subset a a (b1 + 1#64) b2 := by
   revert h
   simp_all [mem_subset_and_mem_subset_for_auto, le_and_bitvec_le, lt_and_bitvec_lt]
-  auto d[mem_subset_for_auto]
+  sorry -- auto d[mem_subset_for_auto]
 
-set_option auto.smt.savepath "/tmp/mem_subset_same_address_different_sizes.smt2" in
+-- set_option auto.smt.savepath "/tmp/mem_subset_same_address_different_sizes.smt2" in
 theorem mem_subset_same_address_different_sizes
   (h : mem_subset addr (addr + n1) addr (addr + n2)) :
   n1 <= n2 := by
   revert h
   simp [mem_subset_and_mem_subset_for_auto, le_and_bitvec_le]
-  auto d[mem_subset_for_auto]
+  sorry -- auto d[mem_subset_for_auto]
 
-set_option auto.smt.savepath "/tmp/first_address_is_subset_of_region.smt2" in
+-- set_option auto.smt.savepath "/tmp/first_address_is_subset_of_region.smt2" in
 theorem first_address_is_subset_of_region :
   mem_subset a a a (a + n) := by
   simp [mem_subset_and_mem_subset_for_auto]
-  auto d[mem_subset_for_auto]
+  sorry -- auto d[mem_subset_for_auto]
 
-set_option auto.smt.savepath "/tmp/first_address_add_one_is_subset_of_region.smt2" in
+-- set_option auto.smt.savepath "/tmp/first_address_add_one_is_subset_of_region.smt2" in
 theorem first_address_add_one_is_subset_of_region (n : Nat) (addr : BitVec 64)
   (_h_lb : 0 < n) (h_ub : n < 2 ^ 64) :
   mem_subset (addr + 1#64) (addr + n#64) addr (addr + n#64) := by
@@ -202,10 +209,10 @@ theorem first_address_add_one_is_subset_of_region (n : Nat) (addr : BitVec 64)
   -- we evaluate it here.
   have : (2^64 = 0x10000000000000000) := by decide
   simp [this] at h_ub
-  auto d[mem_subset_for_auto]
+  sorry -- auto d[mem_subset_for_auto]
 
-set_option auto.smt.timeout 30 in
-set_option auto.smt.savepath "/tmp/first_addresses_add_one_is_subset_of_region_general.smt2" in
+-- set_option auto.smt.timeout 30 in
+-- set_option auto.smt.savepath "/tmp/first_addresses_add_one_is_subset_of_region_general.smt2" in
 theorem first_addresses_add_one_is_subset_of_region_general
   (h0 : 0 < m) (h1 : m < 2 ^ 64) (h2 : n < 2 ^ 64)
   (h3 : mem_subset addr1 (addr1 + m#64) addr2 (addr2 + n#64)) :
@@ -216,16 +223,14 @@ theorem first_addresses_add_one_is_subset_of_region_general
   simp_all [this]
   revert h3
   simp [mem_subset_and_mem_subset_for_auto]
-  auto d[mem_subset_for_auto]
+  sorry -- auto d[mem_subset_for_auto]
 
-set_option auto.smt.savepath "/tmp/first_addresses_add_one_preserves_subset_same_addr_helper.smt2" in
+-- set_option auto.smt.savepath "/tmp/first_addresses_add_one_preserves_subset_same_addr_helper.smt2" in
 private theorem first_addresses_add_one_preserves_subset_same_addr_helper (h1l : 0#64 < m) :
   m - 1#64 ≤ (2 ^ 64 - 1)#64 - 1#64 := by
   revert h1l
   simp [lt_and_bitvec_lt, le_and_bitvec_le]
-  have : (2 ^ 64 - 1) = 18446744073709551615 := by decide
-  simp [this]
-  auto
+  sorry -- auto
 
 theorem first_addresses_add_one_preserves_subset_same_addr
   (h1l : 0 < m) (h1u : m < 2 ^ 64)
@@ -260,8 +265,8 @@ theorem first_addresses_add_one_preserves_subset_same_addr
       simp [BitVec.bitvec_to_nat_of_nat, Nat.mod_eq_of_lt]
       · rw [Nat.mod_eq_of_lt h1u]
         rw [Nat.mod_eq_of_lt h2u]
-        rw [Nat.mod_eq_of_lt (by exact tsub_lt_of_lt h1u)]
-        rw [Nat.mod_eq_of_lt (by exact tsub_lt_of_lt h2u)]
+        rw [Nat.mod_eq_of_lt (by omega)]
+        rw [Nat.mod_eq_of_lt (by omega)]
         exact Nat.sub_le_sub_right h3_0 1
       · simp [BitVec.bitvec_to_nat_of_nat, Nat.mod_eq_of_lt, h2u]
         exact h2l
@@ -271,24 +276,24 @@ theorem first_addresses_add_one_preserves_subset_same_addr
     rw [BitVec.add_sub_add_left]
     simp [BitVec.zero_le_sub]
 
-set_option auto.smt.savepath "/tmp/mem_subset_one_addr_region_lemma.smt2" in
+-- set_option auto.smt.savepath "/tmp/mem_subset_one_addr_region_lemma.smt2" in
 theorem mem_subset_one_addr_region_lemma (addr1 addr2 : BitVec 64) (h : n1 <= 2 ^ 64) :
   mem_subset addr1 (addr1 + n1#64 - 1#64) addr2 addr2 → (n1 = 1) ∧ (addr1 = addr2) := by
   simp (config := {ground := true}) at h
   revert h
   simp [mem_subset_and_mem_subset_for_auto]
-  auto d[mem_subset_for_auto]
+  sorry -- auto d[mem_subset_for_auto]
 
-set_option auto.smt.savepath "/tmp/mem_subset_one_addr_region_lemma_alt.smt2" in
+-- set_option auto.smt.savepath "/tmp/mem_subset_one_addr_region_lemma_alt.smt2" in
 theorem mem_subset_one_addr_region_lemma_alt (addr1 addr2 : BitVec 64)
   (h : n1 < 2 ^ 64) :
   mem_subset addr1 (addr1 + n1#64) addr2 addr2 → (n1 = 0) ∧ (addr1 = addr2) := by
   simp (config := {ground := true}) at h
   revert h
   simp [mem_subset_and_mem_subset_for_auto]
-  auto d[mem_subset_for_auto]
+  sorry -- auto d[mem_subset_for_auto]
 
-set_option auto.smt.savepath "/tmp/mem_subset_same_region_lemma.smt2" in
+-- set_option auto.smt.savepath "/tmp/mem_subset_same_region_lemma.smt2" in
 theorem mem_subset_same_region_lemma
   (h0 : 0 < n)
   (h1 : Nat.succ n ≤ 2 ^ 64) :
@@ -296,12 +301,12 @@ theorem mem_subset_same_region_lemma
   simp (config := {ground := true}) at h1
   revert h0 h1
   simp [mem_subset_and_mem_subset_for_auto, le_and_bitvec_le]
-  auto d[mem_subset_for_auto]
+  sorry -- auto d[mem_subset_for_auto]
 
 -- (FIXME) This is a theorem; see
 -- Arm/mem_separate_for_subset.smt2. This can be solved by z3 in ~10s
 -- if only lean-auto would map Lean definitions to SMT definitions.
-set_option auto.smt.savepath "/tmp/mem_subset_trans.smt2" in
+-- set_option auto.smt.savepath "/tmp/mem_subset_trans.smt2" in
 theorem mem_subset_trans
   (h1 : mem_subset a1 a2 b1 b2)
   (h2 : mem_subset b1 b2 c1 c2) :
@@ -314,50 +319,46 @@ theorem mem_subset_trans
 ----------------------------------------------------------------------
 ---- mem_separate ----
 
-set_option auto.smt.savepath "/tmp/mem_separate_commutative.smt2" in
+-- set_option auto.smt.savepath "/tmp/mem_separate_commutative.smt2" in
 theorem mem_separate_commutative :
   mem_separate a1 a2 b1 b2 = mem_separate b1 b2 a1 a2 := by
   simp [mem_separate, mem_overlap_and_mem_overlap_for_auto]
-  auto d[mem_overlap_for_auto]
+  sorry -- auto d[mem_overlap_for_auto]
 
-set_option auto.smt.savepath "/tmp/mem_separate_starting_addresses_neq.smt2" in
+-- set_option auto.smt.savepath "/tmp/mem_separate_starting_addresses_neq.smt2" in
 theorem mem_separate_starting_addresses_neq :
   mem_separate a1 a2 b1 b2 → a1 ≠ b1 := by
   simp [mem_separate, mem_overlap_and_mem_overlap_for_auto]
-  auto d[mem_overlap_for_auto]
+  sorry -- auto d[mem_overlap_for_auto]
 
-set_option auto.smt.savepath "/tmp/mem_separate_neq.smt2" in
+-- set_option auto.smt.savepath "/tmp/mem_separate_neq.smt2" in
 theorem mem_separate_neq :
   a ≠ b ↔ mem_separate a a b b := by
   simp [mem_separate, mem_overlap_and_mem_overlap_for_auto]
-  auto d[mem_overlap_for_auto]
+  sorry -- auto d[mem_overlap_for_auto]
 
-set_option auto.smt.savepath "/tmp/mem_separate_first_addresses_separate.smt2" in
+-- set_option auto.smt.savepath "/tmp/mem_separate_first_addresses_separate.smt2" in
 theorem mem_separate_first_address_separate (h : mem_separate a b c d) :
   mem_separate a a c d := by
   revert h
   simp [mem_separate, mem_overlap_and_mem_overlap_for_auto, lt_and_bitvec_lt]
-  auto d[mem_overlap_for_auto]
+  sorry -- auto d[mem_overlap_for_auto]
 
-set_option auto.smt.savepath "/tmp/mem_separate_contiguous_regions.smt2" in
+-- set_option auto.smt.savepath "/tmp/mem_separate_contiguous_regions.smt2" in
 theorem mem_separate_contiguous_regions (a k n : BitVec 64)
   (hn : n < ((Std.BitVec.ofNat 64 (2^64 - 1)) - k)) :
   mem_separate a (a + k) (a + k + 1#64) (a + k + 1#64 + n) := by
   revert hn
   simp [mem_separate, mem_overlap_and_mem_overlap_for_auto, lt_and_bitvec_lt]
-  have h' : (2 ^ 64 - 1)#64 = 18446744073709551615#64 := by rfl
-  simp [h']
-  auto d[mem_overlap_for_auto]
+  sorry -- auto d[mem_overlap_for_auto]
 
 -- TODO: Perhaps use/modify mem_separate_contiguous_regions instead?
-set_option auto.smt.savepath "/tmp/mem_separate_contiguous_regions_one_address.smt2" in
+-- set_option auto.smt.savepath "/tmp/mem_separate_contiguous_regions_one_address.smt2" in
 theorem mem_separate_contiguous_regions_one_address (addr : BitVec 64) (h : n' < 2 ^ 64) :
   mem_separate addr addr (addr + 1#64) (addr + 1#64 + (n' - 1)#64) := by
   revert h
   simp [mem_separate, mem_overlap_and_mem_overlap_for_auto, lt_and_bitvec_lt]
-  have h' : (2 ^ 64) = 18446744073709551616 := by rfl
-  simp [h']
-  auto d[mem_overlap_for_auto]
+  sorry -- auto d[mem_overlap_for_auto]
 
 ----------------------------------------------------------------------
 ---- mem_subset and mem_separate -----
@@ -384,7 +385,7 @@ theorem mem_separate_contiguous_regions_one_address (addr : BitVec 64) (h : n' <
 -- we'd be able to prove this theorem here.
 -- Also note that mem_separate_for_subset2 is somehow easier to prove
 -- than mem_separate_for_subset1 using SMT solvers.
-set_option auto.smt.savepath "/tmp/mem_separate_for_subset2.smt2" in
+-- set_option auto.smt.savepath "/tmp/mem_separate_for_subset2.smt2" in
 -- set_option trace.auto.smt.printCommands true in
 -- set_option trace.Meta.synthInstance true in
 theorem mem_separate_for_subset2
