Proofs/MultiInsts.lean
@@ -4,32 +4,33 @@ Released under Apache 2.0 license as described in the file LICENSE.
 Author(s): Shilpi Goel
 -/
 import Arm.Exec
+import Arm.Util
 import Tactics.Sym
-import Auto
+-- import Auto
 
 section multi_insts_proofs
 
 open Std.BitVec
 
-set_option auto.smt true
-set_option auto.smt.trust true
+-- set_option auto.smt true
+-- set_option auto.smt.trust true
 -- set_option trace.auto.smt.printCommands true
 -- set_option trace.auto.smt.result true
 -- set_option auto.proofReconstruction false
 
 def test_program : program :=
   def_program
-  #[(0x12650c#64 , 0x4ea01c1a#32),      --  mov     v26.16b, v0.16b
+  [(0x12650c#64 , 0x4ea01c1a#32),      --  mov     v26.16b, v0.16b
     (0x126510#64 , 0x4ea11c3b#32),      --  mov     v27.16b, v1.16b
     (0x126514#64 , 0x4ea21c5c#32),      --  mov     v28.16b, v2.16b
     (0x126518#64 , 0x4ea31c7d#32)]      --  mov     v29.16b, v3.16b
 
 theorem one_asm_snippet_sym_helper1 (q0_var : BitVec 128) :
   zeroExtend 128 (zeroExtend 128 (zeroExtend 128 q0_var ||| zeroExtend 128 q0_var)) = zeroExtend 128 q0_var := by
-  auto
+  sorry -- auto
 
 theorem one_asm_snippet_sym_helper2 (q0_var : BitVec 128) :
-  q0_var ||| q0_var = q0_var := by auto
+  q0_var ||| q0_var = q0_var := by sorry -- auto
 
 theorem small_asm_snippet_sym (s : ArmState)
   (h_pc : read_pc s = 0x12650c#64)
@@ -38,6 +39,7 @@ theorem small_asm_snippet_sym (s : ArmState)
   (h_s' : s' = run 4 s) :
   read_sfp 128 26#5 s' = read_sfp 128 0#5 s ∧
   read_err s' = StateError.None := by
+    FIXME
     -- iterate 4 (sym1 [h_program])
     sym1 [h_program]
     sym1 [h_program]
@@ -46,7 +48,7 @@ theorem small_asm_snippet_sym (s : ArmState)
     -- Wrapping up the result:
     -- generalize (r (StateField.SFP 0#5) s) = q0_var; unfold state_value at q0_var; simp at q0_var
     -- try (simp [one_asm_snippet_sym_helper1])
-    simp only [one_asm_snippet_sym_helper2]    
+    simp only [one_asm_snippet_sym_helper2]
     done
 
 end multi_insts_proofs
